Also rename msubst to consistent names

src/PlutusIR/Semantics/Dynamic/AnnotationSubstitution.v
@@ -16,7 +16,7 @@ Local Open Scope string_scope.
 Section SubstABindings.
   Context {substAb : tyname -> Ty -> Binding -> Binding}.
 
-  Fixpoint substituteA_bindings_nonrec (X : tyname) (U : Ty) (bs : list Binding) : list Binding :=
+  Fixpoint substA_bnr' (X : tyname) (U : Ty) (bs : list Binding) : list Binding :=
     match bs with
     | nil => 
         nil
@@ -25,121 +25,124 @@ Section SubstABindings.
           then
             substAb X U b :: bs'
           else
-            substAb X U b :: substituteA_bindings_nonrec X U bs'
+            substAb X U b :: substA_bnr' X U bs'
     end.
 
-  Fixpoint substituteA_bindings_rec (X : tyname) (U : Ty) (bs : list Binding) : list Binding :=
+  Fixpoint substA_br' (X : tyname) (U : Ty) (bs : list Binding) : list Binding :=
     match bs with
     | nil =>
         nil
     | b :: bs' =>
-        substAb X U b :: substituteA_bindings_rec X U bs'
+        substAb X U b :: substA_br' X U bs'
     end.
 
 End SubstABindings.
 
 Section SubstAConstructors.
 
-  Definition substituteA_constructor (X : tyname) (U : Ty) (c : constructor) : constructor :=
+  Definition substA_c (X : tyname) (U : Ty) (c : constructor) : constructor :=
     match c with
     | Constructor (VarDecl bx T) ar =>
         Constructor (VarDecl bx (substituteT X U T)) ar
     end.
 
-  Definition substituteA_constructors (X : tyname) (U : Ty) (cs : list constructor) : list constructor :=
-    map (substituteA_constructor X U) cs.
+  Definition substA_cs (X : tyname) (U : Ty) (cs : list constructor) : list constructor :=
+    map (substA_c X U) cs.
 
 End SubstAConstructors.
 
 
-Fixpoint substituteA (X : tyname) (U : Ty) (t : Term) {struct t} : Term :=
+Fixpoint substA (X : tyname) (U : Ty) (t : Term) {struct t} : Term :=
   match t with
   | Let NonRec bs t0 =>
-      Let NonRec (@substituteA_bindings_nonrec substituteA_binding X U bs)
+      Let NonRec (@substA_bnr' substA_b X U bs)
         (if existsb (eqb X) (btvbs bs) 
           then t0
-          else substituteA X U t0
+          else substA X U t0
         ) 
   | Let Rec bs t0 =>
       if existsb (eqb X) (btvbs bs) 
         then 
           Let Rec bs t0
         else
-          Let Rec (@substituteA_bindings_rec substituteA_binding X U bs) (substituteA X U t0)
+          Let Rec (@substA_br' substA_b X U bs) (substA X U t0)
   | Var y => 
       Var y
   | TyAbs bX K t0 =>
       if X =? bX
         then TyAbs bX K t0
-        else TyAbs bX K (substituteA X U t0)
+        else TyAbs bX K (substA X U t0)
   | LamAbs bx T t0 =>
-      LamAbs bx (substituteT X U T) (substituteA X U t0)
+      LamAbs bx (substituteT X U T) (substA X U t0)
   | Apply t1 t2 =>
-      Apply (substituteA X U t1) (substituteA X U t2)
+      Apply (substA X U t1) (substA X U t2)
   | Constant u =>
       Constant u
   | Builtin d =>
       Builtin d
   | TyInst t0 T =>
-      TyInst (substituteA X U t0) (substituteT X U T)
+      TyInst (substA X U t0) (substituteT X U T)
   | Error T =>
       Error (substituteT X U T)
   | IWrap F T t0 =>
-      IWrap (substituteT X U F) (substituteT X U T) (substituteA X U t0)
+      IWrap (substituteT X U F) (substituteT X U T) (substA X U t0)
   | Unwrap t0 =>
-      Unwrap (substituteA X U t0)
+      Unwrap (substA X U t0)
   end
 
-with substituteA_binding (X : tyname) (U : Ty) (b : Binding) {struct b} : Binding :=
+with substA_b (X : tyname) (U : Ty) (b : Binding) {struct b} : Binding :=
   match b with
   | TermBind stricty (VarDecl y T) tb =>
-      TermBind stricty (VarDecl y (substituteT X U T)) (substituteA X U tb)
+      TermBind stricty (VarDecl y (substituteT X U T)) (substA X U tb)
   | TypeBind tvd T => 
       TypeBind tvd (substituteT X U T)
   | DatatypeBind (Datatype tvd YKs matchFunc cs) =>
-      DatatypeBind (Datatype tvd YKs matchFunc (substituteA_constructors X U cs))
+      DatatypeBind (Datatype tvd YKs matchFunc (substA_cs X U cs))
   end.
 
-Notation "'[[' U '/' X ']' t" := (substituteA X U t) (in custom plutus_term at level 20, X constr).
-Notation "'[[' U '/' X '][b]' b" := (substituteA_binding X U b) (in custom plutus_term at level 20, X constr).
-Notation "'[[' U '/' X '][bnr]' bs" := (@substituteA_bindings_nonrec substituteA_binding X U bs) (in custom plutus_term at level 20, X constr).
-Notation "'[[' U '/' X '][br]' bs" := (@substituteA_bindings_rec substituteA_binding X U bs) (in custom plutus_term at level 20, X constr).
-Notation "'[[' U '/' X '][cs]' cs" := (substituteA_constructors X U cs) (in custom plutus_term at level 20, X constr).
-Notation "'[[' U '/' X '][c]' c" := (substituteA_constructor X U c) (in custom plutus_term at level 20, X constr).
+Definition substA_bnr X U bs := @substA_bnr' substA_b X U bs.
+Definition substA_br X U bs := @substA_br' substA_b X U bs.
+
+Notation "'[[' U '/' X ']' t" := (substA X U t) (in custom plutus_term at level 20, X constr).
+Notation "'[[' U '/' X '][b]' b" := (substA_b X U b) (in custom plutus_term at level 20, X constr).
+Notation "'[[' U '/' X '][bnr]' bs" := (substA_bnr X U bs) (in custom plutus_term at level 20, X constr).
+Notation "'[[' U '/' X '][br]' bs" := (substA_br X U bs) (in custom plutus_term at level 20, X constr).
+Notation "'[[' U '/' X '][cs]' cs" := (substA_cs X U cs) (in custom plutus_term at level 20, X constr).
+Notation "'[[' U '/' X '][c]' c" := (substA_c X U c) (in custom plutus_term at level 20, X constr).
 
 (** Multi-substitutions of types in type annotations *)
-Fixpoint msubstA_term (ss : list (tyname * Ty)) (t : Term) : Term :=
+Fixpoint msubstA (ss : list (tyname * Ty)) (t : Term) : Term :=
   match ss with
   | nil => t
-  | (X, U) :: ss' => msubstA_term ss' <{ [[U / X] t }>
+  | (X, U) :: ss' => msubstA ss' <{ [[U / X] t }>
   end.
 
-Fixpoint msubstA_binding (ss : list (tyname * Ty)) (b : Binding) : Binding :=
+Fixpoint msubstA_b (ss : list (tyname * Ty)) (b : Binding) : Binding :=
   match ss with
   | nil => b
-  | (X, U) :: ss' => msubstA_binding ss' <{ [[U / X][b] b }>
+  | (X, U) :: ss' => msubstA_b ss' <{ [[U / X][b] b }>
   end.
 
-Fixpoint msubstA_bindings_nonrec (ss : list (tyname * Ty)) (bs : list Binding) : list Binding :=
+Fixpoint msubstA_bnr (ss : list (tyname * Ty)) (bs : list Binding) : list Binding :=
   match ss with
   | nil => bs
-  | (X, U) :: ss' => msubstA_bindings_nonrec ss' <{ [[U / X][bnr] bs }>
+  | (X, U) :: ss' => msubstA_bnr ss' <{ [[U / X][bnr] bs }>
   end.
 
-Fixpoint msubstA_bindings_rec (ss : list (tyname * Ty)) (bs : list Binding) : list Binding :=
+Fixpoint msubstA_br (ss : list (tyname * Ty)) (bs : list Binding) : list Binding :=
   match ss with
   | nil => bs
-  | (X, U) :: ss' => msubstA_bindings_rec ss' <{ [[U / X][br] bs }>
+  | (X, U) :: ss' => msubstA_br ss' <{ [[U / X][br] bs }>
   end.
 
-Fixpoint msubstA_constructors (ss : list (tyname * Ty)) (cs : list constructor) : list constructor :=
+Fixpoint msubstA_cs (ss : list (tyname * Ty)) (cs : list constructor) : list constructor :=
   match ss with
   | nil => cs
-  | (X, U) :: ss' => msubstA_constructors ss' <{ [[U / X][cs] cs}>
+  | (X, U) :: ss' => msubstA_cs ss' <{ [[U / X][cs] cs}>
   end.
 
-Notation "'/[[' ss '/]' t" := (msubstA_term ss t) (in custom plutus_term at level 20, ss constr).
-Notation "'/[[' ss '/][b]' b" := (msubstA_binding ss b) (in custom plutus_term at level 20, ss constr).
-Notation "'/[[' ss '/][bnr]' bs" := (msubstA_bindings_nonrec ss bs) (in custom plutus_term at level 20, ss constr).
-Notation "'/[[' ss '/][cs]' cs" := (msubstA_constructors ss cs) (in custom plutus_term at level 20, ss constr).
+Notation "'/[[' ss '/]' t" := (msubstA ss t) (in custom plutus_term at level 20, ss constr).
+Notation "'/[[' ss '/][b]' b" := (msubstA_b ss b) (in custom plutus_term at level 20, ss constr).
+Notation "'/[[' ss '/][bnr]' bs" := (msubstA_bnr ss bs) (in custom plutus_term at level 20, ss constr).
+Notation "'/[[' ss '/][cs]' cs" := (msubstA_cs ss cs) (in custom plutus_term at level 20, ss constr).
   
